theories/Languages/Imp.v
@@ -1,4 +1,5 @@
 From Reactive Require Import Base.
+From Reactive.Datatypes Require Dict.
 
 
 Inductive type :=
@@ -35,3 +36,60 @@ Record method := mk_method {
 
   m_body: stmt;
 }.
+
+
+(** ** Semantics *)
+
+Inductive value :=
+  | VConst : const -> value
+  | VInput : binder -> value
+  | VBinop : binop -> value -> value -> value.
+
+Definition stack := Dict.t value.
+
+Inductive sem_exp: stack -> exp -> value -> Prop :=
+  | SeConst (s: stack) (c: const):
+      sem_exp s (EConst c) (VConst c)
+
+  | SeInput (s: stack) (b: binder):
+      sem_exp s (EInput b) (VInput b)
+
+  | SeVar (s: stack) (b: binder) (v: value):
+      Dict.maps_to (fst b) v s ->
+      sem_exp s (EVar b) v
+
+  | SeBinop (s: stack) (op: binop) (e1 e2: exp) (v1 v2: value):
+      sem_exp s e1 v1 ->
+      sem_exp s e2 v2 ->
+      sem_exp s (EBinop op e1 e2) (VBinop op v1 v2).
+
+Inductive sem_stmt: stack -> stmt -> stack -> Prop :=
+  | SeAssign (s: stack) (name: ident) (e: exp) (v: value):
+      sem_exp s e v ->
+      sem_stmt s (SAssign name e) (Dict.add name v s)
+
+  | SeSeq (s1 s2 s3: stack) (st1 st2: stmt):
+      sem_stmt s1 st1 s2 ->
+      sem_stmt s2 st2 s3 ->
+      sem_stmt s1 (SSeq st1 st2) s3
+
+  | SeReturn (s: stack) (e: exp) (v: value):
+      sem_exp s e v ->
+      sem_stmt s (SReturn e) s
+
+  | SeNop (s: stack):
+      sem_stmt s SNop s.
+
+Fixpoint eval_exp (e: exp) (s: stack): option value :=
+  match e with
+    | EConst c => Some (VConst c)
+    | EInput b => Some (VInput b)
+    | EVar (name, typ) => Dict.find name s
+    | EBinop op e1 e2 => match eval_exp e1 s, eval_exp e2 s with
+      | Some v1, Some v2 => Some (VBinop op v1 v2)
+      | _, _ => None
+    end
+  end.
+
+Definition is_evaluable (e: exp) (s: stack): Prop :=
+  exists v: value, eval_exp e s = Some v.
